@prefix owl: <http://www.w3.org/2002/07/owl#> .
@prefix rdf: <http://www.w3.org/1999/02/22-rdf-syntax-ns#> .
@prefix xsd: <http://www.w3.org/2001/XMLSchema#> .
@prefix occp: <http://www.semanticweb.org/albrechtvaatz/ontologies/2022/9/cMod_V0.1#> .
@prefix rdfs: <http://www.w3.org/2000/01/rdf-schema#> .
@base <http://www.semanticweb.org/albrechtvaatz/ontologies/2022/9/cMod_V0.1> .
@prefix sh:     <http://www.w3.org/ns/shacl#> .
@prefix time:   <http://www.w3.org/2006/time#> .
@prefix osh:    <http://www.occpshape.de/shape#> .

<http://www.semanticweb.org/albrechtvaatz/ontologies/2022/9/cMod_V0.1> rdf:type owl:Ontology ;
                                                                        owl:imports <http://www.w3.org/2006/time#> ;
                                                                        rdfs:comment "First workaround to implement time tracking features to models"@en .

#################################################################
#    Object Properties
#################################################################

	###  http://www.semanticweb.org/albrechtvaatz/ontologies/2022/9/cMod_V0.1#after
	occp:after rdf:type owl:ObjectProperty ;
		rdfs:subPropertyOf time:after ;
		owl:inverseOf occp:before ;
		rdfs:domain <http://www.w3.org/2006/time#TemporalEntity> ;
		rdfs:range <http://www.w3.org/2006/time#TemporalEntity> ;
		rdf:type owl:TransitiveProperty ;
		rdfs:comment "This property represents a transitive relation between temporal entities, used to ensure that if A occurs after B and B occurs after C, then A occurs after C."@en ;
		rdfs:label "after (transitive)"@en .


	###  http://www.semanticweb.org/albrechtvaatz/ontologies/2022/9/cMod_V0.1#before
	occp:before rdf:type owl:ObjectProperty ;
		rdfs:subPropertyOf time:before ;
		owl:inverseOf occp:after ;
		rdfs:domain <http://www.w3.org/2006/time#TemporalEntity> ;
		rdfs:range <http://www.w3.org/2006/time#TemporalEntity> ;
		rdf:type owl:TransitiveProperty ;
		rdfs:comment "This property represents a transitive relation between temporal entities, used to ensure that if A occurs before B and B occurs before C, then A occurs before C."@en ;
		rdfs:label "before (transitive)"@en .


	###  http://www.semanticweb.org/albrechtvaatz/ontologies/2022/9/cMod_V0.1#beginsAfter
	occp:beginsAfter rdf:type owl:ObjectProperty ;
		rdfs:subPropertyOf <http://www.w3.org/2006/time#hasBeginning> ;
		rdfs:domain <http://www.w3.org/2006/time#Interval> ;
		rdfs:range <http://www.w3.org/2006/time#TemporalEntity> ;
		owl:inverseOf occp:beginsBefore ;
		rdf:type owl:TransitiveProperty ;
		rdfs:comment "This property represents the chronological order of beginnings between two temporal entities, used to indicate that T1’s beginning occurs after T2’s beginning, without defining the order of their ends."@en ;
		rdfs:label "begins after"@en .


	###  http://www.semanticweb.org/albrechtvaatz/ontologies/2022/9/cMod_V0.1#beginsBefore
	occp:beginsBefore rdf:type owl:ObjectProperty ;
		rdfs:subPropertyOf <http://www.w3.org/2006/time#hasBeginning> ;
		rdfs:domain <http://www.w3.org/2006/time#Interval> ;
		rdfs:range <http://www.w3.org/2006/time#TemporalEntity> ;
		owl:inverseOf occp:beginsAfter ;
		rdf:type owl:TransitiveProperty ;
		rdfs:comment "This property represents the chronological order of beginnings between two temporal entities, used to indicate that T1’s beginning occurs before T2’s beginning, without defining the order of their ends."@en ;
		rdfs:label "begins before"@en .


	###  http://www.semanticweb.org/albrechtvaatz/ontologies/2022/9/cMod_V0.1#beginsWith
	occp:beginsWith rdf:type owl:ObjectProperty ;
		rdfs:subPropertyOf <http://www.w3.org/2006/time#hasBeginning> ;
		rdfs:domain <http://www.w3.org/2006/time#Interval> ;
		rdfs:range <http://www.w3.org/2006/time#TemporalEntity> ;
		rdfs:comment "This property represents the chronological order of beginnings between two temporal entities, used to indicate that T1’s beginning occurs on the same day as T2’s beginning, without defining the order of their ends."@en ;
		rdfs:label "begins with"@en .


	###  http://www.semanticweb.org/albrechtvaatz/ontologies/2022/9/cMod_V0.1#belongsToLifeCycle							
	occp:belongsToLifeCycle rdf:type owl:ObjectProperty ;
		rdfs:domain time:TemporalEntity ;
		rdfs:range occp:LifeCycle ;
		rdfs:comment "This property represents the connection of a phase or instant to its lifecycle, used to link temporal entities to the overarching lifecycle they belong to."@en ;
		rdfs:label "belongs to lifecycle"@en .								


	###  http://www.semanticweb.org/albrechtvaatz/ontologies/2022/9/cMod_V0.1#endsAfter
	occp:endsAfter rdf:type owl:ObjectProperty ;
		rdfs:subPropertyOf <http://www.w3.org/2006/time#hasEnd> ;
		rdfs:domain <http://www.w3.org/2006/time#Interval> ;
		rdfs:range <http://www.w3.org/2006/time#TemporalEntity> ;
		owl:inverseOf occp:endsBefore ;
		rdf:type owl:TransitiveProperty ;
		rdfs:comment "This property represents the chronological order of endings between two temporal entities, used to indicate that T1’s end occurs after T2’s end, without defining the order of their beginnings."@en ;
		rdfs:label "ends after"@en .


	###  http://www.semanticweb.org/albrechtvaatz/ontologies/2022/9/cMod_V0.1#endsBefore
	occp:endsBefore rdf:type owl:ObjectProperty ;
		rdfs:subPropertyOf <http://www.w3.org/2006/time#hasEnd> ;
		rdfs:domain <http://www.w3.org/2006/time#Interval> ;
		rdfs:range <http://www.w3.org/2006/time#TemporalEntity> ;
		owl:inverseOf occp:endsAfter ;
		rdf:type owl:TransitiveProperty ;
		rdfs:comment "This property represents the chronological order of endings between two temporal entities, used to indicate that T1’s end occurs before T2’s end, without defining the order of their beginnings."@en ;
		rdfs:label "ends before"@en .


	###  http://www.semanticweb.org/albrechtvaatz/ontologies/2022/9/cMod_V0.1#endsCycle
	occp:endsCycle rdf:type owl:ObjectProperty ;
		rdfs:subPropertyOf <http://www.w3.org/2006/time#hasEnd> ;
		rdfs:domain <http://www.w3.org/2006/time#Instant> ;
		rdfs:range occp:Cycle ;
		rdfs:comment "This property represents the relationship between an instant and a cycle, used to mark instants that end an ongoing cycle within a phase."@en ;
		rdfs:label "ends cycle"@en .


	###  http://www.semanticweb.org/albrechtvaatz/ontologies/2022/9/cMod_V0.1#endsPhase
	occp:endsPhase rdf:type owl:ObjectProperty ;
		rdfs:subPropertyOf <http://www.w3.org/2006/time#hasEnd> ;
		rdfs:domain <http://www.w3.org/2006/time#Instant> ;
		rdfs:range occp:Phase ;
		rdfs:comment "This property represents the relationship between an instant and a phase, used to mark instants that end an ongoing phase."@en ;
		rdfs:label "ends phase"@en .


	###  http://www.semanticweb.org/albrechtvaatz/ontologies/2022/9/cMod_V0.1#endsWith
	occp:endsWith rdf:type owl:ObjectProperty ;
		rdfs:subPropertyOf <http://www.w3.org/2006/time#hasEnd> ;
		rdfs:domain <http://www.w3.org/2006/time#Interval> ;
		rdfs:range <http://www.w3.org/2006/time#TemporalEntity> ;
		rdfs:comment "This property represents the chronological order of endings between two temporal entities, used to indicate that T1’s end occurs on the same day as T2’s end, without defining the order of their beginnings."@en ;
		rdfs:label "ends with"@en .


	###  http://www.semanticweb.org/albrechtvaatz/ontologies/2022/9/cMod_V0.1#hasActualBeginning
	occp:hasActualBeginning rdf:type owl:ObjectProperty ;
		rdfs:subPropertyOf <http://www.w3.org/2006/time#hasBeginning> ;
		rdfs:domain <http://www.w3.org/2006/time#Interval> ;
		rdfs:range <http://www.w3.org/2006/time#Instant> ;
		rdfs:comment "This property represents the connection between an interval and an instant, used to mark the actual beginning of a phase."@en ;
		rdfs:label "has actual beginning"@en .


    ###  http://www.semanticweb.org/albrechtvaatz/ontologies/2022/9/cMod_V0.1#hasActualEnd
    occp:hasActualEnd rdf:type owl:ObjectProperty ;
		rdfs:subPropertyOf <http://www.w3.org/2006/time#hasEnd> ;
		rdfs:domain <http://www.w3.org/2006/time#Interval> ;
		rdfs:range  <http://www.w3.org/2006/time#Instant> ;
		rdfs:comment "This property represents the connection between an interval and an instant, used to mark the actual end of a phase."@en ;
		rdfs:label "has actual end"@en .


    ###  http://www.semanticweb.org/albrechtvaatz/ontologies/2022/9/cMod_V0.1#hasActualTime
    occp:hasActualTime rdf:type owl:ObjectProperty ;
		rdfs:subPropertyOf <http://www.w3.org/2006/time#hasTime> ;
		rdfs:domain <http://www.w3.org/2006/time#Instant> ;
		rdfs:range  xsd:date ;
		rdfs:comment "This property represents the connection between an instant and a date, used to mark the actual point in time of an instant."@en ;
		rdfs:label "has actual time"@en .


    ###  http://www.semanticweb.org/albrechtvaatz/ontologies/2022/9/cMod_V0.1#hasCycleNumber
    occp:hasCycleNumber rdf:type owl:DatatypeProperty ;
		rdfs:domain occp:Cycle ;
		rdfs:range xsd:integer ;
		rdfs:comment "This property represents the number of iterations in a cycle, used to specify how many times a process like a planning review repeats (e.g., in CycleA_PlanningReview)."@en ;
		rdfs:label "has cycle number"@en .


    ###  http://www.semanticweb.org/albrechtvaatz/ontologies/2022/9/cMod_V0.1#hasEstimatedBeginning
    occp:hasEstimatedBeginning rdf:type owl:ObjectProperty ;
		rdfs:subPropertyOf <http://www.w3.org/2006/time#hasBeginning> ;
		rdfs:domain <http://www.w3.org/2006/time#Interval> ;
		rdfs:range  <http://www.w3.org/2006/time#Instant> ;
		rdfs:comment "This property represents the connection between an interval and an instant, used to mark the estimated beginning of a phase."@en ;
		rdfs:label "has estimated beginning"@en .


    ###  http://www.semanticweb.org/albrechtvaatz/ontologies/2022/9/cMod_V0.1#hasEstimatedEnd
    occp:hasEstimatedEnd rdf:type owl:ObjectProperty ;
		rdfs:subPropertyOf <http://www.w3.org/2006/time#hasEnd> ;
		rdfs:domain <http://www.w3.org/2006/time#Interval> ;
		rdfs:range  <http://www.w3.org/2006/time#Instant> ;
		rdfs:comment "This property represents the connection between an interval and an instant, used to mark the estimated end of a phase."@en ;
		rdfs:label "has estimated end"@en .


    ###  http://www.semanticweb.org/albrechtvaatz/ontologies/2022/9/cMod_V0.1#hasEstimatedTime
    occp:hasEstimatedTime rdf:type owl:ObjectProperty ;
		rdfs:subPropertyOf <http://www.w3.org/2006/time#hasTime> ;
		rdfs:domain <http://www.w3.org/2006/time#Instant> ;
		rdfs:range  xsd:date ;
		rdfs:comment "This property represents the connection between an instant and a date, used to mark the estimated point in time of an instant."@en ;
		rdfs:label "has estimated time"@en .


    ###  http://www.semanticweb.org/albrechtvaatz/ontologies/2022/9/cMod_V0.1#hasInstant
    occp:hasInstant rdf:type owl:ObjectProperty ;
		rdfs:range <http://www.w3.org/2006/time#Instant> ;
		rdfs:comment "This property represents the link between an updatable entity and an instant, used to connect specific lifecycle events (e.g., Submission) from the MsOCCP to components or models."@en ;
		rdfs:label "has instant"@en .


    ###  http://www.semanticweb.org/albrechtvaatz/ontologies/2022/9/cMod_V0.1#hasLifecycle
    occp:hasLifecycle a rdf:Property ;
        rdfs:domain occp:Site ;
        rdfs:range occp:Lifecycle ;
        rdfs:comment "Links a site to the lifecycles of buildings constructed on it." ;
        rdfs:label "hasLifecycle" .


    ###  http://www.semanticweb.org/albrechtvaatz/ontologies/2022/9/cMod_V0.1#hasPhase
    occp:hasPhase rdf:type owl:ObjectProperty ;
		rdfs:domain <http://www.w3.org/2006/time#Instant> ;
		rdfs:range occp:Phase ;
		rdfs:comment "This property represents the connection between an instant and a phase, used to link time instants to their respective phases."@en ;
		rdfs:label "has phase"@en .


    ###  http://www.semanticweb.org/albrechtvaatz/ontologies/2022/9/cMod_V0.1#isInPhase
    occp:isInPhase rdf:type owl:ObjectProperty ;
		rdfs:domain occp:LifeCycle ;
		rdfs:range occp:Phase ;
		rdfs:comment "This property represents the embedding of a lifecycle within a phase, used to link a lifecycle to the overarching phase it belongs to."@en ;
		rdfs:label "is in phase"@en .


    ###  http://www.semanticweb.org/albrechtvaatz/ontologies/2022/9/cMod_V0.1#startsCycle
    occp:startsCycle rdf:type owl:ObjectProperty ;
		rdfs:subPropertyOf <http://www.w3.org/2006/time#hasBeginning> ;
		rdfs:domain <http://www.w3.org/2006/time#Instant> ;
		rdfs:range occp:Cycle ;
		rdfs:comment "This property represents the relationship between an instant and a cycle, used to mark instants that start a new cycle within a phase."@en ;
		rdfs:label "starts cycle"@en .


    ###  http://www.semanticweb.org/albrechtvaatz/ontologies/2022/9/cMod_V0.1#startsPhase
    occp:startsPhase rdf:type owl:ObjectProperty ;
		rdfs:subPropertyOf <http://www.w3.org/2006/time#hasBeginning> ;
		rdfs:domain <http://www.w3.org/2006/time#Instant> ;
		rdfs:range occp:Phase ;
		rdfs:comment "This property represents the relationship between an instant and a phase, used to mark instants that start a new phase."@en ;
		rdfs:label "starts phase"@en . 


#################################################################
#    Datatype Properties
#################################################################

	###  http://www.semanticweb.org/albrechtvaatz/ontologies/2022/9/cMod_V0.1#hasLifeCycleID
	occp:hasLifeCycleID rdf:type owl:DatatypeProperty ;
		rdfs:domain occp:LifeCycle ;
		rdfs:range xsd:string ;
		rdfs:comment "This property represents the unique identifier of a lifecycle, used to provide a distinct ID for tracking purposes."@en ;
		rdfs:label "has lifecycle ID"@en .


#################################################################
#    Classes
#################################################################

    ###  http://www.semanticweb.org/albrechtvaatz/ontologies/2022/9/cMod_V0.1#BeginOfTenderingProcess
    occp:BeginOfTenderingProcess rdf:type owl:Class ;
		rdfs:subClassOf occp:Transition ;
		rdfs:comment "This class represents the instant marking the start of the tendering process, a transition between the planning and construction phases, occurring after the completion of planning."@en ;
		rdfs:label "Begin of Tendering Process"@en .


    ###  http://www.semanticweb.org/albrechtvaatz/ontologies/2022/9/cMod_V0.1#BeginningOfPlanning
    occp:BeginningOfPlanning rdf:type owl:Class ;
		rdfs:subClassOf occp:PhaseA_Instant ;
		rdfs:comment "This class represents the instant marking the official start of the planning phase."@en ;
		rdfs:label "Beginning of Planning"@en .


    ###  http://www.semanticweb.org/albrechtvaatz/ontologies/2022/9/cMod_V0.1#CompletionOfConstruction
    occp:CompletionOfConstruction rdf:type owl:Class ;
		rdfs:subClassOf occp:Transition ;
		rdfs:comment "This class represents the instant marking the last acceptance and finish of construction works, serving as a transition between the construction and usage phases."@en ;
		rdfs:label "Completion of Construction"@en .


    ###  http://www.semanticweb.org/albrechtvaatz/ontologies/2022/9/cMod_V0.1#CompletionOfDeconstruction
    occp:CompletionOfDeconstruction rdf:type owl:Class ;
		rdfs:subClassOf occp:Transition ;
		rdfs:comment "This class represents the instant marking the completion of the final deconstruction task, ending the lifecycle of a building or construction."@en ;
		rdfs:label "Completion of Deconstruction"@en .


    ###  http://www.semanticweb.org/albrechtvaatz/ontologies/2022/9/cMod_V0.1#CompletionOfPlanning
    occp:CompletionOfPlanning rdf:type owl:Class ;
		rdfs:subClassOf occp:Transition ;
		rdfs:comment "This class represents the instant marking the last planning review acceptance, serving as a transition from the planning phase to the tendering process."@en ;
		rdfs:label "Completion of Planning"@en .


    ###  http://www.semanticweb.org/albrechtvaatz/ontologies/2022/9/cMod_V0.1#ConstructionAcceptance
    occp:ConstructionAcceptance rdf:type owl:Class ;
		rdfs:subClassOf occp:PhaseC_Instant ;
		rdfs:comment "This class represents the instant marking the final acceptance of a construction or component, occurring after completion or defect elimination."@en ;
		rdfs:label "Construction Acceptance"@en .


    ###  http://www.semanticweb.org/albrechtvaatz/ontologies/2022/9/cMod_V0.1#ConstructionCompletion
    occp:ConstructionCompletion rdf:type owl:Class ;
		rdfs:subClassOf occp:PhaseC_Instant ;
		rdfs:comment "This class represents the instant marking the completion of construction for a model component or building."@en ;
		rdfs:label "Construction Completion"@en .


    ###  http://www.semanticweb.org/albrechtvaatz/ontologies/2022/9/cMod_V0.1#ConstructionStart
    occp:ConstructionStart rdf:type owl:Class ;
		rdfs:subClassOf occp:PhaseC_Instant ;
		rdfs:comment "This class represents the instant marking the beginning of construction works for a model component or building."@en ;
		rdfs:label "Construction Start"@en .


    ###  http://www.semanticweb.org/albrechtvaatz/ontologies/2022/9/cMod_V0.1#Cycle
    occp:Cycle rdf:type owl:Class ;
		rdfs:subClassOf <http://www.w3.org/2006/time#Interval> ;
		rdfs:comment "This class represents a recurring time span with a starting point, period, and duration, used to track iterating processes like multiple planning reviews."@en ;
		rdfs:label "Cycle"@en .


    ###  http://www.semanticweb.org/albrechtvaatz/ontologies/2022/9/cMod_V0.1#CycleA_PlanningReview
    occp:CycleA_PlanningReview rdf:type owl:Class ;
		rdfs:subClassOf occp:Cycle ;
		rdfs:comment "This class represents a cycle starting with plan submission and ending with approval or rejection, used to track planning and review iterations. Multiple events possible if rejected."@en ;
		rdfs:label "Cycle A Planning Review"@en .


    ###  http://www.semanticweb.org/albrechtvaatz/ontologies/2022/9/cMod_V0.1#DamageDetection
    occp:DamageDetection rdf:type owl:Class ;
		rdfs:subClassOf occp:PhaseK_Instant ;
		rdfs:comment "This class represents the instant marking the detection of damage affecting a component or building. Multiple events possible."@en ;
		rdfs:label "Damage Detection"@en .


    ###  http://www.semanticweb.org/albrechtvaatz/ontologies/2022/9/cMod_V0.1#DamageObservation
    occp:DamageObservation rdf:type owl:Class ;
		rdfs:subClassOf occp:PhaseK_Instant ;
		rdfs:comment "This class represents the instant marking the observation of a known defect or damage, typically linked to inspections or monitoring systems. Multiple events possible."@en ;
		rdfs:label "Damage Observation"@en .


    ###  http://www.semanticweb.org/albrechtvaatz/ontologies/2022/9/cMod_V0.1#DamageRepair
    occp:DamageRepair rdf:type owl:Class ;
		rdfs:subClassOf occp:PhaseK_Instant ;
		rdfs:comment "This class represents the instant marking the repair of a defect or damage, typically coinciding with the end of repair measures."@en ;
		rdfs:label "Damage Repair"@en .


    ###  http://www.semanticweb.org/albrechtvaatz/ontologies/2022/9/cMod_V0.1#DataProcurement
    occp:DataProcurement rdf:type owl:Class ;
		rdfs:subClassOf occp:PhaseA_Instant ;
		rdfs:comment "This class represents the instant marking data procurement actions, such as geodetic measures or adding data to planning models. Multiple events possible."@en ;
		rdfs:label "Data Procurement"@en .


    ###  http://www.semanticweb.org/albrechtvaatz/ontologies/2022/9/cMod_V0.1#DeconstructionCompletion
    occp:DeconstructionCompletion rdf:type owl:Class ;
		rdfs:subClassOf occp:PhaseM_Instant ;
		rdfs:comment "This class represents the instant marking the completion of deconstruction works, ending the lifecycle of a component or building."@en ;
		rdfs:label "Deconstruction Completion"@en .


    ###  http://www.semanticweb.org/albrechtvaatz/ontologies/2022/9/cMod_V0.1#DeconstructionStart
    occp:DeconstructionStart rdf:type owl:Class ;
		rdfs:subClassOf occp:PhaseM_Instant ;
		rdfs:comment "This class represents the instant marking the beginning of deconstruction works for a component or building."@en ;
		rdfs:label "Deconstruction Start"@en .


    ###  http://www.semanticweb.org/albrechtvaatz/ontologies/2022/9/cMod_V0.1#DefectElimCompletion
    occp:DefectElimCompletion rdf:type owl:Class ;
		rdfs:subClassOf occp:PhaseC_Instant ;
		rdfs:comment "This class represents the instant marking the completion of construction works related to defect elimination for a model component or building."@en ;
		rdfs:label "Defect Elimination Completion"@en .


    ###  http://www.semanticweb.org/albrechtvaatz/ontologies/2022/9/cMod_V0.1#DefectElimStart
    occp:DefectElimStart rdf:type owl:Class ;
		rdfs:subClassOf occp:PhaseC_Instant ;
		rdfs:comment "This class represents the instant marking the beginning of construction works related to defect elimination for a model component or building."@en ;
		rdfs:label "Defect Elimination Start"@en .


    ###  http://www.semanticweb.org/albrechtvaatz/ontologies/2022/9/cMod_V0.1#DesignLifeChange
    occp:DesignLifeChange rdf:type owl:Class ;
		rdfs:subClassOf occp:PhaseF_Instant ;
		rdfs:comment "This class represents the instant marking a change in the estimated design life due to factors like repairs or usage changes. Multiple events possible."@en ;
		rdfs:label "Design Life Change"@en .


    ###  http://www.semanticweb.org/albrechtvaatz/ontologies/2022/9/cMod_V0.1#DesignLifeEnd
    occp:DesignLifeEnd rdf:type owl:Class ;
		rdfs:subClassOf occp:PhaseF_Instant ;
		rdfs:comment "This class represents the instant marking the end of the estimated design life of a component or building. Multiple events possible due to estimation changes."@en ;
		rdfs:label "Design Life End"@en .


    ###  http://www.semanticweb.org/albrechtvaatz/ontologies/2022/9/cMod_V0.1#DesignLifeStart
    occp:DesignLifeStart rdf:type owl:Class ;
		rdfs:subClassOf occp:PhaseF_Instant ;
		rdfs:comment "This class represents the instant marking the start of the estimated design life of a component or building."@en ;
		rdfs:label "Design Life Start"@en .


    ###  http://www.semanticweb.org/albrechtvaatz/ontologies/2022/9/cMod_V0.1#Edit_ASTR
    occp:Edit_ASTR rdf:type owl:Class ;
		rdfs:subClassOf occp:PhaseA_Instant ;
		rdfs:comment "This class represents the instant marking significant changes to a planning model after submission to review (ASTR = After Submission To Review). Multiple events possible."@en ;
		rdfs:label "Edit ASTR"@en .


    ###  http://www.semanticweb.org/albrechtvaatz/ontologies/2022/9/cMod_V0.1#Edit_BSTR
    occp:Edit_BSTR rdf:type owl:Class ;
		rdfs:subClassOf occp:PhaseA_Instant ;
		rdfs:comment "This class represents the instant marking significant changes to a planning model before submission to review (BSTR = Before Submission To Review). Multiple events possible."@en ;
		rdfs:label "Edit BSTR"@en .


    ###  http://www.semanticweb.org/albrechtvaatz/ontologies/2022/9/cMod_V0.1#GeologicalEvent
    occp:GeologicalEvent rdf:type owl:Class ;
		rdfs:subClassOf occp:PhaseH_Instant ;
		rdfs:comment "This class represents the instant marking a geological event (e.g., earthquake) affecting a component or building. Multiple events possible."@en ;
		rdfs:label "Geological Event"@en .


    ###  http://www.semanticweb.org/albrechtvaatz/ontologies/2022/9/cMod_V0.1#InspectionExecution
    occp:InspectionExecution rdf:type owl:Class ;
		rdfs:subClassOf occp:PhaseG_Instant ;
		rdfs:comment "This class represents the instant marking the execution of a regular inspection. Multiple events possible over the lifecycle."@en ;
		rdfs:label "Inspection Execution"@en .


    ###  http://www.semanticweb.org/albrechtvaatz/ontologies/2022/9/cMod_V0.1#IrregularInspection
    occp:IrregularInspection rdf:type owl:Class ;
		rdfs:subClassOf occp:PhaseG_Instant ;
		rdfs:comment "This class represents the instant marking the execution of an irregular inspection. Multiple events possible over the lifecycle."@en ;
		rdfs:label "Irregular Inspection"@en .


	###  http://www.semanticweb.org/albrechtvaatz/ontologies/2022/9/cMod_V0.1#LifeCycle		
	occp:LifeCycle rdf:type owl:Class ;
		rdfs:subClassOf time:Interval ;
		rdfs:comment "This class represents a complete lifecycle (Phases A to M) within an overarching phase or another lifecycle, identified by a unique ID."@en ;
		rdfs:label "Life Cycle"@en .


    ###  http://www.semanticweb.org/albrechtvaatz/ontologies/2022/9/cMod_V0.1#LoadEvent
    occp:LoadEvent rdf:type owl:Class ;
		rdfs:subClassOf occp:PhaseH_Instant ;
		rdfs:comment "This class represents the instant marking an irregular load event affecting a component or building. Multiple events possible."@en ;
		rdfs:label "Load Event"@en .


    ###  http://www.semanticweb.org/albrechtvaatz/ontologies/2022/9/cMod_V0.1#NewComponent
    occp:NewComponent rdf:type owl:Class ;
		rdfs:subClassOf occp:PhaseL_Instant ;
		rdfs:comment "This class represents the instant marking the addition of a new component to an existing structure, potentially initiating a sub-lifecycle. Multiple events possible."@en ;
		rdfs:label "New Component"@en .


    ###  http://www.semanticweb.org/albrechtvaatz/ontologies/2022/9/cMod_V0.1#NextRegularInspection
    occp:NextRegularInspection rdf:type owl:Class ;
		rdfs:subClassOf occp:PhaseG_Instant ;
		rdfs:comment "This class represents the instant marking the planned date of the next regular inspection, based on the inspection interval. Multiple events possible over the lifecycle."@en ;
		rdfs:label "Next Regular Inspection"@en .


    ###  http://www.semanticweb.org/albrechtvaatz/ontologies/2022/9/cMod_V0.1#Phase
    occp:Phase rdf:type owl:Class ;
		rdfs:subClassOf <http://www.w3.org/2006/time#Interval> ;
		rdfs:comment "This class represents the main chronological blocks of a building’s lifecycle (e.g., planning, construction, usage), serving as a customizable base structure."@en ;
		rdfs:label "Phase"@en .


    ###  http://www.semanticweb.org/albrechtvaatz/ontologies/2022/9/cMod_V0.1#PhaseA_Instant
    occp:PhaseA_Instant rdf:type owl:Class ;
		rdfs:subClassOf <http://www.w3.org/2006/time#Instant> ;
		rdfs:comment "This class represents instants within Phase A (Planning Phase), grouping all related events."@en ;
		rdfs:label "Phase A Instant"@en .


    ###  http://www.semanticweb.org/albrechtvaatz/ontologies/2022/9/cMod_V0.1#PhaseA_Planning
    occp:PhaseA_Planning rdf:type owl:Class ;
		rdfs:subClassOf occp:Phase ;
		rdfs:comment "This class represents the planning phase, starting with BeginningOfPlanning and ending with CompletionOfPlanning."@en ;
		rdfs:label "Phase A Planning"@en .


    ###  http://www.semanticweb.org/albrechtvaatz/ontologies/2022/9/cMod_V0.1#PhaseB_Instant
    occp:PhaseB_Instant rdf:type owl:Class ;
		rdfs:subClassOf <http://www.w3.org/2006/time#Instant> ;
		rdfs:comment "This class represents instants within Phase B (Review Phase), grouping all related events."@en ;
		rdfs:label "Phase B Instant"@en .


    ###  http://www.semanticweb.org/albrechtvaatz/ontologies/2022/9/cMod_V0.1#PhaseB_Review
    occp:PhaseB_Review rdf:type owl:Class ;
		rdfs:subClassOf occp:Phase ;
		rdfs:comment "This class represents the review phase, starting with the first submission to review and ending with CompletionOfPlanning."@en ;
		rdfs:label "Phase B Review"@en .


    ###  http://www.semanticweb.org/albrechtvaatz/ontologies/2022/9/cMod_V0.1#PhaseC_Construction
    occp:PhaseC_Construction rdf:type owl:Class ;
		rdfs:subClassOf occp:Phase ;
		rdfs:comment "This class represents the construction phase, starting with ConstructionStart and ending with CompletionOfConstruction."@en ;
		rdfs:label "Phase C Construction"@en .


    ###  http://www.semanticweb.org/albrechtvaatz/ontologies/2022/9/cMod_V0.1#PhaseC_Instant
    occp:PhaseC_Instant rdf:type owl:Class ;
		rdfs:subClassOf <http://www.w3.org/2006/time#Instant> ;
		rdfs:comment "This class represents instants within Phase C (Construction Phase), grouping all related events."@en ;
		rdfs:label "Phase C Instant"@en .


    ###  http://www.semanticweb.org/albrechtvaatz/ontologies/2022/9/cMod_V0.1#PhaseD_Instant
    occp:PhaseD_Instant rdf:type owl:Class ;
		rdfs:subClassOf <http://www.w3.org/2006/time#Instant> ;
		rdfs:comment "This class represents instants within Phase D (Usage Phase), grouping all related events."@en ;
		rdfs:label "Phase D Instant"@en .


    ###  http://www.semanticweb.org/albrechtvaatz/ontologies/2022/9/cMod_V0.1#PhaseD_Usage
    occp:PhaseD_Usage rdf:type owl:Class ;
		rdfs:subClassOf occp:Phase ;
		rdfs:comment "This class represents the usage phase, starting with UsageStart and ending with UsageEnd."@en ;
		rdfs:label "Phase D Usage"@en .


    ###  http://www.semanticweb.org/albrechtvaatz/ontologies/2022/9/cMod_V0.1#PhaseE_Instant
    occp:PhaseE_Instant rdf:type owl:Class ;
		rdfs:subClassOf <http://www.w3.org/2006/time#Instant> ;
		rdfs:comment "This class represents instants within Phase E (Warranty Phase), grouping all related events."@en ;
		rdfs:label "Phase E Instant"@en .


    ###  http://www.semanticweb.org/albrechtvaatz/ontologies/2022/9/cMod_V0.1#PhaseE_Warranty
    occp:PhaseE_Warranty rdf:type owl:Class ;
		rdfs:subClassOf occp:Phase ;
		rdfs:comment "This class represents the warranty phase, starting with WarrantyStart and ending with WarrantyEnd."@en ;
		rdfs:label "Phase E Warranty"@en .


    ###  http://www.semanticweb.org/albrechtvaatz/ontologies/2022/9/cMod_V0.1#PhaseF_DesignLife
    occp:PhaseF_DesignLife rdf:type owl:Class ;
		rdfs:subClassOf occp:Phase ;
		rdfs:comment "This class represents the design life phase, starting with DesignLifeStart and ending with DesignLifeEnd."@en ;
		rdfs:label "Phase F Design Life"@en .


    ###  http://www.semanticweb.org/albrechtvaatz/ontologies/2022/9/cMod_V0.1#PhaseF_Instant
    occp:PhaseF_Instant rdf:type owl:Class ;
		rdfs:subClassOf <http://www.w3.org/2006/time#Instant> ;
		rdfs:comment "This class represents instants within Phase F (Design Life Phase), grouping all related events."@en ;
		rdfs:label "Phase F Instant"@en .


    ###  http://www.semanticweb.org/albrechtvaatz/ontologies/2022/9/cMod_V0.1#PhaseG_Inspection
    occp:PhaseG_Inspection rdf:type owl:Class ;
		rdfs:subClassOf occp:Phase ;
		rdfs:comment "This class represents the inspection phase, starting with the beginning of usage and ending with the beginning of deconstruction."@en ;
		rdfs:label "Phase G Inspection"@en .


    ###  http://www.semanticweb.org/albrechtvaatz/ontologies/2022/9/cMod_V0.1#PhaseG_Instant
    occp:PhaseG_Instant rdf:type owl:Class ;
		rdfs:subClassOf <http://www.w3.org/2006/time#Instant> ;
		rdfs:comment "This class represents instants within Phase G (Inspection Phase), grouping all related events."@en ;
		rdfs:label "Phase G Instant"@en .


    ###  http://www.semanticweb.org/albrechtvaatz/ontologies/2022/9/cMod_V0.1#PhaseH_Instant
    occp:PhaseH_Instant rdf:type owl:Class ;
		rdfs:subClassOf <http://www.w3.org/2006/time#Instant> ;
		rdfs:comment "This class represents instants within Phase H (Special Events Phase), grouping all related events."@en ;
		rdfs:label "Phase H Instant"@en .


    ###  http://www.semanticweb.org/albrechtvaatz/ontologies/2022/9/cMod_V0.1#PhaseH_SpecialEvents
    occp:PhaseH_SpecialEvents rdf:type owl:Class ;
		rdfs:subClassOf occp:Phase ;
		rdfs:comment "This class represents the special events phase, starting with the first special event and ending with the last."@en ;
		rdfs:label "Phase H Special Events"@en .


    ###  http://www.semanticweb.org/albrechtvaatz/ontologies/2022/9/cMod_V0.1#PhaseK_Damage
    occp:PhaseK_Damage rdf:type owl:Class ;
		rdfs:subClassOf occp:Phase ;
		rdfs:comment "This class represents the damage phase, starting with DamageDetection and ending with repair completion or deconstruction start."@en ;
		rdfs:label "Phase K Damage"@en .


    ###  http://www.semanticweb.org/albrechtvaatz/ontologies/2022/9/cMod_V0.1#PhaseK_Instant
    occp:PhaseK_Instant rdf:type owl:Class ;
		rdfs:subClassOf <http://www.w3.org/2006/time#Instant> ;
		rdfs:comment "This class represents instants within Phase K (Damage Phase), grouping all related events."@en ;
		rdfs:label "Phase K Instant"@en .


    ###  http://www.semanticweb.org/albrechtvaatz/ontologies/2022/9/cMod_V0.1#PhaseL_Instant
    occp:PhaseL_Instant rdf:type owl:Class ;
		rdfs:subClassOf <http://www.w3.org/2006/time#Instant> ;
		rdfs:comment "This class represents instants within Phase L (Repair Phase), grouping all related events."@en ;
		rdfs:label "Phase L Instant"@en .


    ###  http://www.semanticweb.org/albrechtvaatz/ontologies/2022/9/cMod_V0.1#PhaseL_Repair
    occp:PhaseL_Repair rdf:type owl:Class ;
		rdfs:subClassOf occp:Phase ;
		rdfs:comment "This class represents the repair phase, starting with RepairStart and ending with RepairCompletion."@en ;
		rdfs:label "Phase L Repair"@en .


    ###  http://www.semanticweb.org/albrechtvaatz/ontologies/2022/9/cMod_V0.1#PhaseM_Deconstruction
    occp:PhaseM_Deconstruction rdf:type owl:Class ;
		rdfs:subClassOf occp:Phase ;
		rdfs:comment "This class represents the deconstruction phase, starting with DeconstructionStart and ending with DeconstructionCompletion."@en ;
		rdfs:label "Phase M Deconstruction"@en .


    ###  http://www.semanticweb.org/albrechtvaatz/ontologies/2022/9/cMod_V0.1#PhaseM_Instant
    occp:PhaseM_Instant rdf:type owl:Class ;
		rdfs:subClassOf <http://www.w3.org/2006/time#Instant> ;
		rdfs:comment "This class represents instants within Phase M (Deconstruction Phase), grouping all related events."@en ;
		rdfs:label "Phase M Instant"@en .


    ###  http://www.semanticweb.org/albrechtvaatz/ontologies/2022/9/cMod_V0.1#RepairCompletion
    occp:RepairCompletion rdf:type owl:Class ;
		rdfs:subClassOf occp:PhaseL_Instant ;
		rdfs:comment "This class represents the instant marking the completion of damage repair works for a component or building. Multiple events possible."@en ;
		rdfs:label "Repair Completion"@en .


    ###  http://www.semanticweb.org/albrechtvaatz/ontologies/2022/9/cMod_V0.1#RepairStart
    occp:RepairStart rdf:type owl:Class ;
		rdfs:subClassOf occp:PhaseL_Instant ;
		rdfs:comment "This class represents the instant marking the beginning of damage repair works for a component or building. Multiple events possible."@en ;
		rdfs:label "Repair Start"@en .


    ###  http://www.semanticweb.org/albrechtvaatz/ontologies/2022/9/cMod_V0.1#ReviewApproval
    occp:ReviewApproval rdf:type owl:Class ;
		rdfs:subClassOf occp:PhaseB_Instant ;
		rdfs:comment "This class represents the instant marking the reviewer’s acceptance of a planning model, ending the planning and review phases."@en ;
		rdfs:label "Review Approval"@en .


    ###  http://www.semanticweb.org/albrechtvaatz/ontologies/2022/9/cMod_V0.1#ReviewRejection
    occp:ReviewRejection rdf:type owl:Class ;
		rdfs:subClassOf occp:PhaseB_Instant ;
		rdfs:comment "This class represents the instant marking the reviewer’s rejection of a planning model. Multiple events possible."@en ;
		rdfs:label "Review Rejection"@en .


    ###  http://www.semanticweb.org/albrechtvaatz/ontologies/2022/9/cMod_V0.1#ReviewStart
    occp:ReviewStart rdf:type owl:Class ;
		rdfs:subClassOf occp:PhaseB_Instant ;
		rdfs:comment "This class represents the instant marking the start of the review process. Multiple events possible with rejections."@en ;
		rdfs:label "Review Start"@en .


    ###  http://www.semanticweb.org/albrechtvaatz/ontologies/2022/9/cMod_V0.1#Site
    occp:Site a rdfs:Class ;
        rdfs:comment "A physical site or parcel of land that serves as a container for lifecycles of buildings." ;
        rdfs:label "Site" .


    ###  http://www.semanticweb.org/albrechtvaatz/ontologies/2022/9/cMod_V0.1#Submission
    occp:Submission rdf:type owl:Class ;
		rdfs:subClassOf occp:Transition ;
		rdfs:comment "This class represents the instant marking the end of the tendering process, serving as a transition to the construction phase."@en ;
		rdfs:label "Submission"@en .


    ###  http://www.semanticweb.org/albrechtvaatz/ontologies/2022/9/cMod_V0.1#SubmissionToReview
    occp:SubmissionToReview rdf:type owl:Class ;
		rdfs:subClassOf occp:PhaseA_Instant ;
		rdfs:comment "This class represents the instant marking the submission of a planning draft to the reviewer, starting Phase B. Multiple events possible."@en ;
		rdfs:label "Submission to Review"@en .


    ###  http://www.semanticweb.org/albrechtvaatz/ontologies/2022/9/cMod_V0.1#Transition
    occp:Transition rdf:type owl:Class ;
		rdfs:subClassOf <http://www.w3.org/2006/time#Instant> ;
		rdfs:comment "This class represents key milestones or triggering events between phases, typically enabling the start of the next phase or marking phase completion."@en ;
		rdfs:label "Transition"@en .


    ###  http://www.semanticweb.org/albrechtvaatz/ontologies/2022/9/cMod_V0.1#UsageChange
    occp:UsageChange rdf:type owl:Class ;
		rdfs:subClassOf occp:PhaseD_Instant ;
		rdfs:comment "This class represents the instant marking a change in usage of a component or building, potentially ending one or more usage phases and initiating new ones. Multiple events possible."@en ;
		rdfs:label "Usage Change"@en .


    ###  http://www.semanticweb.org/albrechtvaatz/ontologies/2022/9/cMod_V0.1#UsageEnd
    occp:UsageEnd rdf:type owl:Class ;
		rdfs:subClassOf occp:PhaseD_Instant ;
		rdfs:comment "This class represents the instant marking the end of usage for a component or building. Multiple events possible."@en ;
		rdfs:label "Usage End"@en .


    ###  http://www.semanticweb.org/albrechtvaatz/ontologies/2022/9/cMod_V0.1#UsageStart
    occp:UsageStart rdf:type owl:Class ;
		rdfs:subClassOf occp:PhaseD_Instant ;
		rdfs:comment "This class represents the instant marking the beginning of usage for a component or building. Multiple events possible."@en ;
		rdfs:label "Usage Start"@en .


    ###  http://www.semanticweb.org/albrechtvaatz/ontologies/2022/9/cMod_V0.1#WarrantyChange
    occp:WarrantyChange rdf:type owl:Class ;
		rdfs:subClassOf occp:PhaseE_Instant ;
		rdfs:comment "This class represents the instant marking a change in warranty due to repairs or extensions. Multiple events possible."@en ;
		rdfs:label "Warranty Change"@en .


    ###  http://www.semanticweb.org/albrechtvaatz/ontologies/2022/9/cMod_V0.1#WarrantyEnd
    occp:WarrantyEnd rdf:type owl:Class ;
		rdfs:subClassOf occp:PhaseE_Instant ;
		rdfs:comment "This class represents the instant marking the end of a warranty period for a component or building. Multiple events possible due to restarts."@en ;
		rdfs:label "Warranty End"@en .


    ###  http://www.semanticweb.org/albrechtvaatz/ontologies/2022/9/cMod_V0.1#WarrantyStart
    occp:WarrantyStart rdf:type owl:Class ;
		rdfs:subClassOf occp:PhaseE_Instant ;
		rdfs:comment "This class represents the instant marking the beginning of a warranty period for a component or building. Multiple events possible due to restarts."@en ;
		rdfs:label "Warranty Start"@en .


    ###  http://www.semanticweb.org/albrechtvaatz/ontologies/2022/9/cMod_V0.1#WeatherEvent
    occp:WeatherEvent rdf:type owl:Class ;
		rdfs:subClassOf occp:PhaseH_Instant ;
		rdfs:comment "This class represents the instant marking a weather event (e.g., flood) affecting a component or building. Multiple events possible."@en ;
		rdfs:label "Weather Event"@en .


